Linking openssl

code/experimental/he/hestarhs/exec/Main.hs
@@ -5,6 +5,8 @@ import Universum
 import Playground
 import TestHacl
 
+
+
 main :: IO ()
 main = do
     print =<< genDataDGK [(31,1)] 512
