code/experimental/rsapss/include/Hacl_Impl_Bignum_Openssl.h
@@ -1,0 +1,9 @@
+#include "kremlib.h"
+
+void Hacl_Impl_Bignum_Openssl_ossl_mod_exp(
+  uint32_t nLen,
+  uint32_t expLen,
+  uint64_t *n,
+  uint64_t *a,
+  uint64_t *b,
+  uint64_t *res);
